Added documentation

src/Core.Environment.fst
@@ -4,6 +4,9 @@ open Util.Reader
 
 open Core.Ltt
 
+(**
+Represents a declaration.
+*)
 type decl =
   | Function : term : ltt -> ty : ltt -> decl
 
@@ -18,13 +21,26 @@ type env = list (name * decl)
 
 (** Look up a declaration within the typechecking
     environment. *)
-val env_lookup : env -> name -> option decl
+abstract val env_lookup : env -> name -> option decl
 let rec env_lookup e n =
   match e with
   | [] -> None
   | (sn,sd) :: xs -> if sn = n
       then Some sd
       else env_lookup xs n
+
+(**
+`env_add` adds a declaration to an environment.
+*)
+abstract val env_add : env -> name -> decl -> env
+let env_add e n d = (n,d) :: e
+
+(**
+`env_init` initializes an environment using a
+list of tuples pairing a name and a declaration.
+*)
+abstract val env_init : list (name * decl) -> env
+let env_init = id
 
 (** The base effect that typechecking occurs within. *)
 total reifiable reflectable new_effect TC = READER env
@@ -33,19 +49,27 @@ total reifiable reflectable new_effect TC = READER env
 effect Tc (a:Type) (pre:TC?.pre) (post:env -> a -> GTot Type0) =
   TC a (fun l0 p -> pre l0 /\ (forall x. pre l0 /\ post l0 x ==> p x))
 
+(** Utility effect for trivial conditions for the `TC` effect. *)
 effect TcNull (a:Type) =
   TC a (fun (e0:env) (p:(a -> Type0)) -> forall (x:a). p x)
 
+(** Read the typechecking environment *)
 val read : unit -> TcNull env
 let read = TC?.get
 
+(** Lookup a declaration in the typechecking environment. *)
 val lookup : name -> TcNull (option decl)
 let lookup n =
   let e = read () in
   env_lookup e n
 
+(**
+Lookup the value associated with a name in the typechecking
+environment.
+*)
 val lookup_term : name -> TcNull (option ltt)
 let lookup_term n =
   match lookup n with
   | Some (Function t _) -> Some t
   | _ -> None
+
