TODO.md
@@ -1,5 +1,4 @@
 # TODO
-1. add docs for everything
-2. add `Exn` to the `Tc` monad
-3. implement weak head normal form
-4. implement `equate`
+1. add `Exn` to the `Tc` monad
+2. implement weak head normal form
+3. implement `equate`
